feat: equivalence of iterators (#8545)
This PR provides the means to reason about "equivalent" iterators.
Simply speaking, two iterators are equivalent if they behave the same as
long as consumers do not introspect their states.

src/Std/Data/Iterators/Lemmas/Combinators/FilterMap.lean
@@ -181,7 +181,7 @@ theorem Iter.step_mapM {f : β → n γ}
     match it.step with
     | .yield it' out h => do
       let out' ← f out
-      pure <| .yield (it'.mapM f) out' (.yieldSome h ⟨_, rfl⟩)
+      pure <| .yield (it'.mapM f) out' (.yieldSome h ⟨⟨out', True.intro⟩, rfl⟩)
     | .skip it' h =>
       pure <| .skip (it'.mapM f) (.skip h)
     | .done h =>
@@ -220,7 +220,7 @@ theorem Iter.step_filterMap {f : β → Option γ} :
   · simp
   · simp
 
-def Iter.step_map {f : β → γ} :
+theorem Iter.step_map {f : β → γ} :
     (it.map f).step = match it.step with
       | .yield it' out h =>
         .yield (it'.map f) (f out) (.yieldSome (out := out) h ⟨⟨f out, rfl⟩, rfl⟩)
