src/Std/Data/Iterators/Producers/Monadic/Array.lean
@@ -23,12 +23,20 @@ variable {α : Type w} {m : Type w → Type w'}
 The underlying state of a list iterator. Its contents are internal and should
 not be used by downstream users of the library.
 -/
-@[unbox]
+@[unbox, ext]
 structure ArrayIterator (α : Type w) where
   /-- Internal implementation detail of the iterator library. -/
   array : Array α
   /-- Internal implementation detail of the iterator library. -/
   pos : Nat
+
+theorem ArrayIterator.exists_iff {α : Type w} {P : ArrayIterator α → Prop} :
+    (∃ s, P s) ↔ ∃ array pos, P ⟨array, pos⟩ := by
+  constructor
+  · rintro ⟨⟨array, pos⟩, h⟩
+    exact ⟨array, pos, h⟩
+  · rintro ⟨array, pos, h⟩
+    exact ⟨⟨array, pos⟩, h⟩
 
 /--
 Returns a finite monadic iterator for the given array starting at the given index.
@@ -41,7 +49,7 @@ The pure version of this iterator is `Array.iterFromIdx`.
 * `Finite` instance: always
 * `Productive` instance: always
 -/
-@[always_inline, inline]
+@[always_inline, inline, match_pattern]
 def _root_.Array.iterFromIdxM {α : Type w} (array : Array α) (m : Type w → Type w') (pos : Nat)
     [Pure m] :
     IterM (α := ArrayIterator α) m α :=
